VertexSet and EdgeSet are sets now

push-relabel/_build/default/bin/.main.eobjs/dune__exe__Main.impl.d
@@ -1,1 +1,1 @@
-bin/main.ml: Format Hashtbl Int List Obj Printf Set Stdlib Sys
+bin/main.ml: Format Hashtbl Int List Obj Printf Seq Set Stdlib Sys
